coq/Examples/ConversionNegator.v
@@ -87,7 +87,7 @@ Section FunctionalSpecification.
     Definition fs_transitions
         (act: fs_action)
         :
-        (tf_ops)
+        (@tf_ops fs_states fs_inputs fs_outputs tf_no_externs)
         :=
         match act with
         | fs_act_nop => tf_ops_base (tf_nop)
@@ -96,7 +96,7 @@ Section FunctionalSpecification.
         | fs_act_write => tf_ops_base (tf_assign fs_st_val (tf_ivar fs_in_val))
         end.
 
-    Definition fs_step := tf_ops_run fs_states_size fs_inputs_size fs_outputs_size.
+    Definition fs_step := tf_ops_run (externs := tf_no_externs_sig) fs_states_size fs_inputs_size fs_outputs_size.
 
     Section Examples.
         (* In the initial state "s_init" the "fs_st_val" is zero *)
@@ -172,6 +172,9 @@ Section TypedSynthesis.
         tfs_spec_outputs := fs_outputs;
         tfs_spec_outputs_fin := _;
         tfs_spec_outputs_size := fs_outputs_size;
+
+        tfs_spec_externs := tf_no_externs;
+        tfs_spec_externs_sig := tf_no_externs_sig;
 
         tfs_spec_action := fs_action;
         tfs_spec_action_fin := _;
